\documentclass{article}
\usepackage{graphicx}

\begin{document}

\title{Introduction to \LaTeX{}}
\author{Author's Name}

\maketitle

Fix a structure $\mathfrak{A} $  and an assignment function $s : Vars \to A $. We have to show: $\mathfrak{U} \models \left( \left[ \left( x_1= y_1 \right) \land \left( x_1= y_1 \right) \land  \dotsb \land \left( x_n= y_n \right)   \right] \to  \left( f\left(x_{1}, x_{2},  \dots ,x_{n - 1},x_{n} \right) = f\left(x_{1}, x_{2},  \dots ,x_{n - 1},x_{n} \right)  \right)  \right) \left[ s \right]$

Since the is an implication of the form $\psi \to  \lambda$  one may assume $\psi$, another way to see that is by looking at the equivalence to $\neg \psi \lor \lambda$, since if $\mathfrak{A} \models \left( \neg \psi  \right)\left[ s \right]  $, in otherwords $\mathfrak{A} \not \models \psi\left[ s \right]$, then we would already know that $\mathfrak{A}  \models \left( \psi \lor \lambda  \right)\left[ s \right]$, therefore one may assume that $\mathfrak{A} \models \psi\left[ s \right]$ and then show that $\mathfrak{A} \models \lambda\left[ s \right] $.

In our case, we assume that $\mathfrak{A} \models \left[ \left( x_1= y_1 \right) \land \left( x_1= y_1 \right) \land  \dotsb \land \left( x_n= y_n \right)   \right]\left[ s \right] $, now we must show that $\mathfrak{A} \models \left( f\left(x_{1}, x_{2},  \dots ,x_{n - 1},x_{n} \right) = f\left(y_{1}, y_{2},  \dots ,y_{n - 1},y_{n} \right)  \right) \left[ s \right] $, recall from the second clause of the definition of satisfaction, one must show that $\bar{s} \left(f\left(x_{1}, x_{2},  \dots ,x_{n - 1},x_{n} \right) \right) = \bar{s} \left(f\left(y_{1}, y_{2},  \dots ,y_{n - 1},y_{n} \right) \right) $, but that $\bar{s} \left(f\left(x_{1}, x_{2},  \dots ,x_{n - 1},x_{n} \right) \right) = f\left(\bar{s} \left( x \right) _{1}, \bar{s} \left( x \right) _{2},  \dots ,\bar{s} \left( x \right) _{n - 1},\bar{s} \left( x \right) _{n} \right) $ and also $\bar{s} \left(f\left(y_{1}, y_{2},  \dots ,y_{n - 1},y_{n} \right) \right) = f\left(\bar{s} \left( y \right) _{1}, \bar{s} \left( y \right) _{2},  \dots ,\bar{s} \left( y \right) _{ n - 1},\bar{s} \left( y \right) _{n} \right) $




\end{document}
